refactor SmallstepClosed

common/SmallstepClosed.v
@@ -7,8 +7,7 @@ Require Import Globalenvs.
 Require Import LanguageInterface.
 Require Import Integers.
 Require Import Smallstep.
-Require Import Compiler.
-Import Values Maps Memory Ctypes AST.
+Import Values Maps Memory AST.
 
 Set Implicit Arguments.
 
@@ -225,8 +224,6 @@ Variable s1 : Smallstep.semantics liA1 liB1.
 Variable se1 : Genv.symtbl.
 Definition lts1 := (Smallstep.activate s1 se1).
 Definition L1 := close_semantics query1 reply1 s1 se1.
-(* Hypothesis closed1 : forall s q, Smallstep.safe lts1 s -> ~ at_external lts1 s q. *)
-(* Hypothesis reply_sound1: forall r, exists i, reply1 i r. *)
 
 Variable liA2 liB2 : language_interface.
 Variable query2 : query liB2.
@@ -235,8 +232,6 @@ Variable s2 : Smallstep.semantics liA2 liB2.
 Variable se2 : Genv.symtbl.
 Definition lts2 := (Smallstep.activate s2 se2).
 Definition L2 := close_semantics query2 reply2 s2 se2.
-Hypothesis closed2 : forall s q, Smallstep.safe lts2 s -> ~ at_external lts2 s q.
-Hypothesis reply_sound2: forall s r, Smallstep.final_state lts2 s r -> exists i, reply2 i r.
 
 Variable ccA : callconv liA1 liA2.
 Variable ccB : callconv liB1 liB2.
@@ -246,19 +241,17 @@ Hypothesis Hvalid : Genv.valid_for (skel s1) se1.
 Variable wB : ccworld ccB.
 
 Hypothesis Hmatch_query : match_query ccB wB query1 query2.
-Hypothesis Hmatch_reply : forall r r1 r2,
-  match_reply ccB wB r1 r2 ->
-  reply1 r r1 <-> reply2 r r2.
-
 Hypothesis Hmatch_senv : match_senv ccB wB se1 se2.
+
+Section FORWARD.
+
+Hypothesis Hmatch_reply_forward : forall r r1 r2,
+  match_reply ccB wB r1 r2 ->
+  reply1 r r1 -> reply2 r r2.
 
 Lemma close_sound_forward :
   Smallstep.forward_simulation ccA ccB s1 s2 -> forward_simulation L1 L2.
 Proof.
-  (* pose proof (Hmatch_query := Hmatch_query).
-  pose proof (Hmatch_reply := Hmatch_reply).
-  pose proof (open_simulation := open_simulation).
-  pose proof (Hvalid := Hvalid). *)
   intro open_simulation.
   unfold Smallstep.forward_simulation in open_simulation.
   inv open_simulation. inv X.
@@ -269,8 +262,12 @@ Proof.
   (* match final state *)
   intros i s1' s2' r MS (r1 & R1 & FINAL).
   exploit fsim_match_final_states0; eauto. intros (r2 & FINAL' & MATCH_REPLY).
-  eexists. split; eauto. eapply Hmatch_reply; eauto.
+  eexists. split; eauto.
 Qed.
+
+End FORWARD.
+
+Section BACKWARD.
 
 Lemma safe_sound_1:
   forall s, safe L1 s -> Smallstep.safe lts1 s.
@@ -278,6 +275,12 @@ Proof.
   unfold safe, Smallstep.safe, L1, lts1, close_semantics. simpl. intros.
   specialize (H _ H0) as [(r & r0 & REPLY & FS)|(t & s'' & STEP)]; eauto.
 Qed.
+
+Hypothesis closed2 : forall s q, Smallstep.safe lts2 s -> ~ at_external lts2 s q.
+Hypothesis reply_sound2: forall s r, Smallstep.final_state lts2 s r -> exists i, reply2 i r.
+Hypothesis Hmatch_reply_backward : forall r r1 r2,
+  match_reply ccB wB r1 r2 ->
+  reply2 r r2 -> reply1 r r1.
 
 Lemma close_sound_backward:
   Smallstep.backward_simulation ccA ccB s1 s2 -> backward_simulation L1 L2.
@@ -297,7 +300,7 @@ Proof.
 
   intros. apply safe_sound_1 in H0. destruct H1 as (r0 & REPLY & FS).
   specialize (bsim_match_final_states0 _ _ _ _ H H0 FS) as (s1' & r1 & STAR & FS' & MS).
-  exists s1'. split; eauto. eexists. split; eauto. eapply Hmatch_reply; eauto.
+  exists s1'. split; eauto.
 
   intros. apply safe_sound_1 in H0.
   pose proof (progress := bsim_progress0).
@@ -310,341 +313,8 @@ Proof.
   eapply bsim_simulation0; eauto.
 Qed.
 
+End BACKWARD.
+
 End CLOSE_SOUND.
-
-Section CLOSE_COMPCERT.
-
-Variable p : Csyntax.program.
-Variable tp : Asm.program.
-Hypothesis transf : transf_c_program p = OK tp.
-Let se := Genv.symboltbl (erase_program p).
-
-Variable main_block_c : block.
-Variable m0_c : mem.
-
-Let liA1 := li_c.
-Let liB1 := li_c.
-Let sg := AST.mksignature nil (AST.Tret AST.Tint) AST.cc_default.
-Let main_function_value_c := Vptr main_block_c Ptrofs.zero.
-Let query1 := cq main_function_value_c sg nil m0_c.
-Inductive reply1 : int -> c_reply -> Prop :=
-  | reply1_intro: forall r m,
-      reply1 r (cr (Vint r) m).
-Let s1 := Csem.semantics p.
-Let se1 := se.
-Let lts1' := (Smallstep.activate s1 se1).
-
-Let ge_c' := Smallstep.globalenv (s1 se).
-Let ge_c := Csem.genv_genv ge_c'.
-Variable main_c : Csyntax.fundef.
-Hypothesis Hinitial_state_c :
-  Genv.init_mem (erase_program p) = Some m0_c /\
-  Genv.find_symbol se p.(prog_main) = Some main_block_c /\
-  Genv.find_funct_ptr ge_c main_block_c = Some main_c.
-
-Import Asm.
-
-Let s2 := Asm.semantics tp.
-Let ge_asm := Smallstep.globalenv (s2 se).
-Variable m0_asm : mem.
-Hypothesis Hinitial_state_asm :
-  Genv.init_mem (erase_program tp) = Some m0_asm.
-
-Let liA2 := li_asm.
-Let liB2 := li_asm.
-Let rs0 :=
-    (Pregmap.init Vundef)
-    # PC <- (Genv.symbol_address ge_asm tp.(prog_main) Ptrofs.zero)
-    # RA <- Vnullptr
-    # RSP <- Vnullptr.
-Let query2 := (rs0, m0_asm).
-Inductive reply2: int -> (regset * mem) -> Prop :=
-  | reply2_intro: forall r rs m,
-      rs#PC = Vnullptr ->
-      rs#RAX = Vint r ->
-      reply2 r (rs, m).
-Let se2 := se.
-Let lts2' := (Smallstep.activate s2 se2).
-
-Ltac clean_destr :=
-  match goal with
-  | H: _ = left _ |- _ => clear H
-  | H: _ = right _ |- _ => clear H
-  end.
-
-Ltac destr :=
-  match goal with
-    |- context [match ?a with _ => _ end] => destruct a eqn:?; try intuition congruence
-  end; repeat clean_destr.
-
-Ltac destr_in H :=
-  match type of H with
-    context [match ?a with _ => _ end] => destruct a eqn:?; try intuition congruence
-  | _ => inv H
-  end; repeat clean_destr.
-
-Lemma erase_same: erase_program p = erase_program tp.
-Proof.
-  exploit transf_c_program_match; eauto. intro MATCH.
-  unfold match_c_prog in MATCH. simpl in MATCH. repeat destruct MATCH as (? & MATCH).
-  fold Csyntax.fundef. remember p as xx.
-  rename xx into p', p into xx. rename p' into p.
-  match goal with
-  | H: ?P p ?p2 |- _ => rewrite Heqxx in H
-  end.
-  rewrite Heqxx. clear Heqxx.
-  Ltac mp H p1 p2 :=
-    unfold Linking.match_program in H;
-    match type of H with
-    | Linking.match_program_gen _ _ _ _ _ =>
-        apply Linking.match_program_skel in H;
-        try fold CminorSel.fundef in H;
-        try fold RTL.fundef in H;
-        rewrite H; clear H p1;
-        rename p2 into p1
-    | Linking.match_program_gen _ _ _ _ _ /\ _ =>
-        let H' := fresh "H" in
-        let garbage := fresh "H" in
-        destruct H as (H' & garbage);
-        clear garbage;
-        mp H' p1 p2
-    end.
-  Ltac try_rewrite xx := match goal with
-  | H: ?P xx ?p2 |- _ =>
-    unfold P in H; mp H xx p2
-  | H: match_if ?cond ?P xx ?p2 |- _ =>
-    unfold match_if, P in H;
-    let H' := fresh "H" in
-    assert (H' : erase_program xx = erase_program p2) by (destr_in H; mp H xx p2; auto);
-    rewrite H';
-    clear H' H xx;
-    rename p2 into xx
-  end.
-  repeat try_rewrite xx.
-  unfold Unusedglobproof.match_prog in H12.
-  destruct H12 as (u & VALID & MATCH').
-  inv MATCH'. rewrite <- match_prog_skel.
-  clear match_prog_main match_prog_public match_prog_def match_prog_skel VALID xx u.
-  rename x12 into xx.
-  repeat try_rewrite xx.
-  auto.
-Qed.
-
-Lemma m0_same: m0_c = m0_asm.
-Proof.
-  rewrite erase_same, Hinitial_state_asm in Hinitial_state_c.
-  destruct Hinitial_state_c. inv H. auto.
-Qed.
-
-Let ccA : callconv liA1 liA2 := cc_compcert.
-Let ccB : callconv liB1 liB2 := cc_compcert.
-
-Lemma Hvalid: Genv.valid_for (erase_program p) se1.
-Proof.
-  red. intros. rewrite Genv.find_info_symbol in H. destruct H as (b & []).
-  exists b, g. unfold se1, se. split; auto. split; auto.
-  destruct g; constructor. constructor.
-  destruct v. constructor; constructor.
-Qed.
-
-Lemma m0_inject: Mem.inject (Mem.flat_inj (Mem.support m0_c)) m0_c m0_asm.
-Proof.
-  rewrite <- m0_same.
-  apply (Genv.initmem_inject (erase_program p)).
-  destruct Hinitial_state_c. auto.
-Qed.
-
-Let wB : ccworld ccB.
-  unfold ccB, cc_compcert, CA.cc_c_asm_injp. simpl.
-  (* ro *)
-  split. split. exact se. split. exact se. exact m0_asm.
-  (* wt_c *)
-  split. split. exact se. split. exact se. exact sg.
-  (* cc_c_asm_injp *)
-  split. split. exact se. split.
-  simpl. econstructor. exact m0_inject. exact sg. exact rs0.
-  (* cc_asm injp *)
-  econstructor. exact m0_inject.
-Defined.
-
-Hypothesis closed:
-  forall v id sg, Genv.find_funct (Genv.globalenv se tp) v <> Some (External (EF_external id sg)).
-
-Lemma closed2 : forall s q, Smallstep.safe lts2' s -> ~ Smallstep.at_external lts2' s q.
-Proof.
-  unfold lts2', s2, se2, semantics. simpl. intros. intro.
-  destruct s. inv H0.
-  eapply closed; eauto.
-Qed.
-
-Lemma reply_sound2: forall s r, Smallstep.final_state lts2' s r -> exists i, reply2 i r.
-Proof.
-  unfold lts2', s2, se2. simpl. intros. destruct s.
-  inversion H.
-  give_up.
-Admitted.
-
-Lemma romem_for_symtbl_sound:
-  ValueAnalysis.romem_for_symtbl se = ValueAnalysis.romem_for p.
-Proof.
-  unfold ValueAnalysis.romem_for, ValueAnalysis.romem_for_symtbl. unfold se.
-  unfold Genv.symboltbl.
-  destruct Hinitial_state_c as (INIT & SYM & FPTR).
-Abort.
-
-Lemma sound_memory_ro: ValueAnalysis.sound_memory_ro se m0_c.
-Proof.
-  unfold se. destruct Hinitial_state_c. clear H0.
-  constructor.
-  apply ValueAnalysis.initial_mem_matches' in H as (? & ? & ? & ROM & ?).
-  2:intros; inv H0; auto.
-  specialize (ROM p ltac:(apply Linking.linkorder_refl)).
-  admit.
-  erewrite Genv.init_mem_genv_sup; eauto.
-Admitted.
-
-Lemma main_block_genv: Genv.find_symbol se (prog_main tp) = Some main_block_c.
-Proof.
-  destruct Hinitial_state_c as [? []].
-  pose proof erase_same. inv H2. simpl in H0. rewrite H0. auto.
-Qed.
-
-Lemma has_main_block: sup_In main_block_c (Mem.support m0_c).
-Proof.
-  destruct Hinitial_state_c as [? []].
-  eapply Genv.find_symbol_not_fresh; eauto.
-Qed.
-
-Lemma Hmatch_query : match_query ccB wB query1 query2.
-Proof.
-  simpl.
-  exists query1. split.
-  constructor. rewrite <- m0_same. constructor. exact sound_memory_ro.
-  exists query1. split.
-  constructor. split. reflexivity. simpl. auto.
-  exists query2. split.
-  unfold query1, query2. econstructor; simpl.
-  unfold Conventions1.loc_arguments. cbn.
-  destruct Archi.ptr64, Archi.win64; simpl; constructor.
-  unfold rs0. simpl.
-  unfold main_function_value_c, Genv.symbol_address.
-  rewrite main_block_genv.
-  econstructor. unfold Mem.flat_inj. pose proof has_main_block. destr.
-  rewrite Ptrofs.add_zero. auto.
-  intros. inv H.
-  cbn. unfold Vnullptr, Tptr. destruct Archi.ptr64; simpl; auto.
-  cbn. unfold Vnullptr, Tptr. destruct Archi.ptr64; simpl; auto.
-  give_up. (* rs0 RSP = Vnullptr *)
-  econstructor.
-  unfold Conventions.tailcall_possible, Conventions.size_arguments, Conventions1.loc_arguments. simpl.
-  destruct Archi.ptr64, Archi.win64; simpl; auto.
-  unfold main_function_value_c. discriminate.
-  discriminate.
-  unfold cc_asm_match'. simpl. split; [|split].
-  intros. unfold rs0.
-  destruct (PregEq.eq r RSP); [subst; rewrite Pregmap.gss|
-  rewrite Pregmap.gso; auto; destruct (PregEq.eq r RA); [subst; rewrite Pregmap.gss|
-  rewrite Pregmap.gso; auto; destruct (PregEq.eq r PC); [subst; rewrite Pregmap.gss|
-  rewrite Pregmap.gso; auto]]].
-  unfold Vnullptr. destr; constructor.
-  unfold Vnullptr. destr; constructor.
-  unfold Genv.symbol_address. destr; econstructor.
-  unfold ge_asm in Heqo. simpl in Heqo. rewrite main_block_genv in Heqo. inv Heqo.
-  unfold Mem.flat_inj. pose proof has_main_block. destr.
-  rewrite Ptrofs.add_zero. auto.
-  unfold rs0.
-  rewrite Pregmap.gso; [|discriminate].
-  rewrite Pregmap.gso; [|discriminate].
-  rewrite Pregmap.gss.
-  unfold ge_asm. simpl. unfold Genv.symbol_address. rewrite main_block_genv. discriminate.
-  rewrite <- m0_same at 2. constructor.
-Admitted.
-
-Lemma Hmatch_reply : forall r r1 r2,
-  match_reply ccB wB r1 r2 ->
-  reply1 r r1 <-> reply2 r r2.
-Proof.
-  simpl. intros.
-  destruct H, H, H0, H0, H1, H1.
-  split; intro r'; inv r'.
-
-  inv H. inv H0. inv H1. inv H2. destruct r2.
-  inv H0. simpl in H2. inv H2.
-  unfold rs0 in H16.
-  rewrite Pregmap.gso in H16; [|discriminate]. rewrite Pregmap.gss in H16.
-  assert (r0 PC = Vnullptr). {
-    pose proof (INJ := H0 PC). rewrite H16 in INJ.
-    unfold Vnullptr. unfold Vnullptr in INJ.
-    destruct Archi.ptr64; inv INJ; auto.
-  }
-  constructor; auto.
-  unfold Conventions1.loc_result, Conventions1.loc_result_64, Conventions1.loc_result_32 in tres.
-  subst tres.
-  destr_in H10; simpl in H10; inv H10;
-  specialize (H0 RAX); rewrite <- H7 in H0; inv H0; auto.
-
-  inv H2. inv H5. destruct x1. simpl in H6. inv H6.
-  specialize (H5 RAX). rewrite H4 in H5. inv H5.
-  inv H1. destruct r1.
-  inv H. destruct H1. inv H0. unfold sg, proj_sig_res in H5. simpl in H5.
-  assert (res = Vint r). {
-    unfold Conventions1.loc_result, Conventions1.loc_result_64, Conventions1.loc_result_32 in tres.
-    subst tres. destr_in H15; simpl in H15.
-    rewrite <- H8 in H15. inv H15. auto.
-    give_up. (* Vundef *)
-    rewrite <- H8 in H15. inv H15. auto.
-    give_up.
-  }
-  subst res. constructor.
-  inv H1. destruct r1.
-  inv H. inv H0.
-  unfold Conventions1.loc_result, Conventions1.loc_result_64, Conventions1.loc_result_32 in tres.
-  subst tres. destr_in H15; simpl in H15; rewrite <- H8 in H15; inv H15.
-  give_up.
-  give_up.
-Admitted.
-
-Lemma Hmatch_senv : match_senv ccB wB se1 se2.
-Proof.
-  unfold ccB, cc_compcert, se1, se2. simpl.
-  split; [|split; [|split]].
-
-  constructor. auto.
-  constructor. auto.
-
-  destruct Hinitial_state_c as (INIT & ? & ?).
-  unfold se. unfold Mem.flat_inj.
-  constructor.
-  split; try erewrite Genv.init_mem_genv_sup by eauto; auto; intros.
-  exists b1. destr.
-  exists b2. destr.
-  1,2,3:destr_in H1.
-  1,2:erewrite Genv.init_mem_genv_sup by eauto. 2:rewrite m0_same.
-  1,2:apply Mem.sup_include_refl.
-
-  destruct Hinitial_state_c as (INIT & ? & ?).
-  unfold se. unfold Mem.flat_inj.
-  constructor.
-  split; try erewrite Genv.init_mem_genv_sup by eauto; auto; intros.
-  exists b1. destr.
-  exists b2. destr.
-  1,2,3:destr_in H1.
-  1,2:erewrite Genv.init_mem_genv_sup by eauto. 2:rewrite m0_same.
-  1,2:apply Mem.sup_include_refl.
-Qed.
-
-Lemma open_simulation: Smallstep.backward_simulation ccA ccB s1 s2.
-Proof.
-  apply c_semantic_preservation, transf_c_program_match. auto.
-Qed.
-
-Lemma compcert_close_sound :
-  backward_simulation (L1 query1 reply1 s1 se1) (L2 query2 reply2 s2 se2).
-Proof.
-  eapply close_sound_backward; eauto using
-    closed2, reply_sound2, Hvalid, Hmatch_query, Hmatch_reply, Hmatch_senv, open_simulation.
-Qed.
-
-End CLOSE_COMPCERT.
 
 End Closed.
